Move semantic path substitution/replacement into dot_lty.v

theories/Dot/lr/dot_lty.v
@@ -2,7 +2,7 @@
 From iris.proofmode Require Import tactics.
 From D Require Export iris_prelude proper lty lr_syn_aux.
 From D.Dot Require Import syn.
-From D.Dot Require Export dlang_inst.
+From D.Dot Require Export dlang_inst path_wp.
 
 Unset Program Cases.
 Set Suggest Proof Using.
@@ -261,3 +261,41 @@ Section logrel_binding_lemmas.
   Lemma interp_subst_commute (T : ty) σ : V⟦ T.|[σ] ⟧ ≡ V⟦ T ⟧.|[σ].
   Proof. intros ???; apply interp_subst_compose_ind. Qed.
 End logrel_binding_lemmas.
+
+(** ** Semantic path substitution and replacement. *)
+
+(** Semantic substitution of path in type. *)
+Definition opSubst `{!dlangG Σ} p (T : oltyO Σ) : oltyO Σ :=
+  Olty (λI args ρ v, path_wp p.|[ρ] (λ w, T args (w .: ρ) v)).
+Notation "T .sTp[ p /]" := (opSubst p T) (at level 65).
+
+(** Semantic definition of path replacement. *)
+Definition sem_ty_path_replI {Σ} p q (T1 T2 : olty Σ) : iProp Σ :=
+  |==> ∀ args ρ v (H : alias_paths p.|[ρ] q.|[ρ]), T1 args ρ v ≡ T2 args ρ v.
+Notation "T1 ~sTpI[ p := q  ]* T2" :=
+  (sem_ty_path_replI p q T1 T2) (at level 70).
+
+(** Semantic definition of path replacement: alternative, weaker version.
+Unlike [sem_ty_path_replI], this version in [Prop] is less expressive, but
+sufficient for our goals and faster to use in certain proofs. *)
+Definition sem_ty_path_repl {Σ} p q (T1 T2 : olty Σ) : Prop :=
+  ∀ args ρ v, alias_paths p.|[ρ] q.|[ρ] → T1 args ρ v ≡ T2 args ρ v.
+Notation "T1 ~sTpP[ p := q  ]* T2" :=
+  (sem_ty_path_repl p q T1 T2) (at level 70).
+
+Section path_repl.
+  Context `{!dlangG Σ}.
+
+  Lemma opSubst_pv_eq v (T : oltyO Σ) : T .sTp[ pv v /] ≡ T.|[v/].
+  Proof. move=> args ρ w /=. by rewrite path_wp_pv_eq subst_swap_base. Qed.
+
+  Lemma sem_psubst_one_repl {T : olty Σ} {args p v w ρ}:
+    alias_paths p.|[ρ] (pv v) →
+    T .sTp[ p /] args ρ w ≡ T args (v .: ρ) w.
+  Proof. move=> /alias_paths_elim_eq /= ->. by rewrite path_wp_pv_eq. Qed.
+
+  Lemma sem_ty_path_repl_eq {p q} {T1 T2 : olty Σ} :
+    T1 ~sTpP[ p := q ]* T2 → ⊢ T1 ~sTpI[ p := q ]* T2.
+  Proof. iIntros "%Heq !% /=". apply: Heq. Qed.
+  (* The reverse does not hold. *)
+End path_repl.
