theories/Dot/lr/dot_semtypes.v
@@ -103,44 +103,6 @@ Section dm_to_type.
   #[global] Opaque dm_to_type.
 End dm_to_type.
 
-(** ** Semantic path substitution and replacement. *)
-
-(** Semantic substitution of path in type. *)
-Definition opSubst `{!dlangG Σ} p (T : oltyO Σ) : oltyO Σ :=
-  Olty (λI args ρ v, path_wp p.|[ρ] (λ w, T args (w .: ρ) v)).
-Notation "T .sTp[ p /]" := (opSubst p T) (at level 65).
-
-(** Semantic definition of path replacement. *)
-Definition sem_ty_path_replI {Σ} p q (T1 T2 : olty Σ) : iProp Σ :=
-  |==> ∀ args ρ v (H : alias_paths p.|[ρ] q.|[ρ]), T1 args ρ v ≡ T2 args ρ v.
-Notation "T1 ~sTpI[ p := q  ]* T2" :=
-  (sem_ty_path_replI p q T1 T2) (at level 70).
-
-(** Semantic definition of path replacement: alternative, weaker version.
-Unlike [sem_ty_path_replI], this version in [Prop] is less expressive, but
-sufficient for our goals and faster to use in certain proofs. *)
-Definition sem_ty_path_repl {Σ} p q (T1 T2 : olty Σ) : Prop :=
-  ∀ args ρ v, alias_paths p.|[ρ] q.|[ρ] → T1 args ρ v ≡ T2 args ρ v.
-Notation "T1 ~sTpP[ p := q  ]* T2" :=
-  (sem_ty_path_repl p q T1 T2) (at level 70).
-
-Section path_repl.
-  Context `{!dlangG Σ}.
-
-  Lemma opSubst_pv_eq v (T : oltyO Σ) : T .sTp[ pv v /] ≡ T.|[v/].
-  Proof. move=> args ρ w /=. by rewrite path_wp_pv_eq subst_swap_base. Qed.
-
-  Lemma sem_psubst_one_repl {T : olty Σ} {args p v w ρ}:
-    alias_paths p.|[ρ] (pv v) →
-    T .sTp[ p /] args ρ w ≡ T args (v .: ρ) w.
-  Proof. move=> /alias_paths_elim_eq /= ->. by rewrite path_wp_pv_eq. Qed.
-
-  Lemma sem_ty_path_repl_eq {p q} {T1 T2 : olty Σ} :
-    T1 ~sTpP[ p := q ]* T2 → ⊢ T1 ~sTpI[ p := q ]* T2.
-  Proof. iIntros "%Heq !% /=". apply: Heq. Qed.
-  (* The reverse does not hold. *)
-End path_repl.
-
 (** ** gDOT semantic types. *)
 Definition vl_sel `{!dlangG Σ} vp l args v : iProp Σ :=
   ∃ d ψ, ⌜vp @ l ↘ d⌝ ∧ d ↗n ψ ∧ packHoLtyO ψ args v.
